src/Computation/SetoidMorphisms.v
@@ -112,6 +112,35 @@ Proof.
   destruct c; eassumption.
 Qed.
 
+Notation "'If' c 'Then' t 'Else' e" :=
+  (If_Then_Else c t e) 
+    (at level 70).
+
+Definition If_Opt_Then_Else {A B}
+           (c : option A)
+           (t : A -> B)
+           (e : B) :=
+  match c with 
+    | Some a => t a
+    | None => e
+  end.
+
+Add Parametric Morphism A B (c : option A)
+: (@If_Opt_Then_Else A (Comp B) c)
+    with signature
+    ((pointwise_relation A (@refine B))
+       ==> @refine B 
+       ==> @refine B )
+      as refine_If_Opt_Then_Else.
+Proof.
+  unfold If_Opt_Then_Else; intros.
+  destruct c; eauto.
+Qed.
+
+Notation "'Ifopt' c 'as' c' 'Then' t 'Else' e" :=
+  (If_Opt_Then_Else c (fun c' => t) e) 
+    (at level 70).
+
 Add Parametric Morphism A
 : (@Pick A)
     with signature
